partial cleanup from misguided attempts

WebAssembly/Wasm_Interpreter_Monad_Properties.thy
@@ -194,201 +194,6 @@ lemma mem_size_triple:"< mi \<mapsto>\<^sub>a mis * list_assn mem_m_assn ms mis 
     
 find_theorems app_s_f_v_s_mem_size
 
-
-definition union_of_disjoint :: "'a set \<Rightarrow> 'a set \<Rightarrow> 'a set option" where 
-  "union_of_disjoint a b = (if a \<inter> b = {} then Some (a \<union> b) else None)"
-
-definition Union_of_disjoint :: "'a set list \<Rightarrow> 'a set option" where 
-  "Union_of_disjoint as = fold (\<lambda>a b. b \<bind> union_of_disjoint a) as (Some {})"
-
-record s_m_vals = 
-  mems_p :: "(byte array \<times> nat option) list"
-  mems_data :: "(byte list \<times> nat option) list" 
-
-definition s_m_vals_agree :: "s_m_vals \<Rightarrow> s \<Rightarrow> bool" where 
- "s_m_vals_agree v s = list_all2 (\<lambda> (bl, n1) (m, n2). bl = Rep_mem_rep m \<and> n1 = n2) 
-    (mems_data v) (s.mems s)" 
-
-definition s_m_assn :: "s_m_vals \<Rightarrow> s_m \<Rightarrow> assn" where
-  "s_m_assn v s_m = s_m.mems s_m \<mapsto>\<^sub>a mems_p v 
-* list_assn (\<lambda> (ba, _) (bl, _ ). ba  \<mapsto>\<^sub>a bl) (mems_p v) (mems_data v)"
-
-definition vals_of_s_m :: "heap \<Rightarrow> s_m \<Rightarrow> (s_m_vals \<times> addr set) option" where 
- "vals_of_s_m h s_m = (
-  let mems_p = Array.get h (s_m.mems s_m) in  
-  (Union_of_disjoint 
-    ({addr_of_array (s_m.mems s_m)} # (map (\<lambda> (ba, _). {addr_of_array ba}) mems_p)))
-  \<bind> (\<lambda>addrs. 
-    Some 
-      (\<lparr>mems_p = mems_p, mems_data = map (\<lambda> (ba, n). (Array.get h ba, n)) mems_p\<rparr>,
-       addrs)))
-"
-
-lemma s_m_vals_sound_assn: 
-  assumes "Some (v, as) = vals_of_s_m h s_m"
-  shows "(h, as) \<Turnstile> s_m_assn v s_m" 
-  sorry
-
-lemma s_m_vals_sound_agree: 
-  assumes "Some (v, as) = vals_of_s_m h s_m"
-  shows "s_m_vals_agree v (s_m_to_s h s_m)"
-  sorry
-
-lemma s_m_preservation:
-  assumes "s_m_vals_agree v s" "(h, as) \<Turnstile> s_m_assn v s_m " 
-  shows "s = s_m_to_s h s_m" 
-  sorry
-
-type_synonym inst_m_vals = inst 
-
-definition inst_m_vals_agree :: "inst_m_vals \<Rightarrow> inst \<Rightarrow> bool" where 
- "inst_m_vals_agree v i = (v = i)" 
-
-definition inst_m_assn :: "inst_m_vals \<Rightarrow> inst_m \<Rightarrow> assn" where
-  "inst_m_assn v i_m = 
-    inst_m.types i_m \<mapsto>\<^sub>a inst.types v
-  * inst_m.funcs i_m \<mapsto>\<^sub>a inst.funcs v  
-  * inst_m.tabs  i_m \<mapsto>\<^sub>a inst.tabs  v 
-  * inst_m.mems  i_m \<mapsto>\<^sub>a inst.mems  v 
-  * inst_m.globs i_m \<mapsto>\<^sub>a inst.globs v"
-
-definition vals_of_inst_m :: "heap \<Rightarrow> inst_m \<Rightarrow> (inst_m_vals \<times> addr set) option" where 
- "vals_of_inst_m h i_m = 
- (Union_of_disjoint 
-  [{addr_of_array (inst_m.types i_m)}, 
-   {addr_of_array (inst_m.funcs i_m)},
-   {addr_of_array (inst_m.tabs  i_m)},
-   {addr_of_array (inst_m.mems  i_m)},
-   {addr_of_array (inst_m.globs i_m)}]) 
- \<bind> (\<lambda>addrs. 
-  Some(\<lparr>
-  inst.types = Array.get h (inst_m.types i_m), 
-  funcs = Array.get h (inst_m.funcs i_m),
-  tabs  = Array.get h (inst_m.tabs i_m), 
-  mems  = Array.get h (inst_m.mems i_m), 
-  globs = Array.get h (inst_m.globs i_m) \<rparr>,
-  addrs) )
-"
-
-lemma inst_m_vals_sound_assn: 
-  assumes "Some (v, as) = vals_of_inst_m h i_m"
-  shows "(h, as) \<Turnstile> inst_m_assn v i_m" 
-  sorry
-
-lemma inst_m_vals_sound_agree: 
-  assumes "Some (v, as) = vals_of_inst_m h i_m"
-  shows "inst_m_vals_agree v (inst_m_to_inst h i_m)"
-  sorry
-
-lemma inst_m_preservation:
-  assumes "inst_m_vals_agree v i" "(h, as) \<Turnstile> inst_m_assn v i_m " 
-  shows "i = inst_m_to_inst h i_m" 
-  sorry
-
-record fc_m_vals = 
-  inst_m_vals :: "inst_m_vals" 
-
-definition fc_m_vals_agree :: "fc_m_vals \<Rightarrow> frame_context \<Rightarrow> bool" where 
- "fc_m_vals_agree v fc = (case fc of Frame_context redex lcs nf f \<Rightarrow>
-  inst_m_vals_agree (inst_m_vals v) (f_inst f)
- )" 
-
-definition fc_m_assn :: "fc_m_vals \<Rightarrow> frame_context_m \<Rightarrow> assn" where
- "fc_m_assn v fc_m = (case fc_m of Frame_context_m redex lcs nf f_locs1 f_inst2 \<Rightarrow> 
-  inst_m_assn (inst_m_vals v) f_inst2
-)" 
-
-definition vals_of_fc_m :: "heap \<Rightarrow> frame_context_m \<Rightarrow> (fc_m_vals \<times> addr set) option" where 
- "vals_of_fc_m h fc_m = (case fc_m of Frame_context_m redex lcs nf f_locs1 f_inst2 \<Rightarrow>
-  (vals_of_inst_m h f_inst2) \<bind>
-  (\<lambda> (inst_m_vals, addrs). 
-  Some (\<lparr>inst_m_vals = inst_m_vals\<rparr>, addrs))
-)"
-
-lemma fc_m_vals_sound_assn: 
-  assumes "Some (v, as) = vals_of_fc_m h fc_m"
-  shows "(h, as) \<Turnstile> fc_m_assn v fc_m" 
-  sorry
-
-lemma fc_m_vals_sound_agree: 
-  assumes "Some (v, as) = vals_of_fc_m h fc_m"
-  shows "fc_m_vals_agree v (frame_context_m_to_frame_context h fc_m)"
-  sorry
-
-lemma fc_m_preservation:
-  assumes "fc_m_vals_agree v fc" "(h, as) \<Turnstile> fc_m_assn v fc_m " 
-  shows "fc = fc_m_to_fc h fc_m" 
-  sorry
-
-lemma fc_m_vals_update_step_m: 
-  "vals_of_fc_m h (update_fc_step_m fc_m v_s' es_cont) = vals_of_fc_m h fc_m"
-  unfolding vals_of_fc_m_def
-  by (simp split: frame_context_m.splits)
-
-record config_m_vals = 
-  s_m_vals :: "s_m_vals"
-  fc_m_vals :: "fc_m_vals"
-  fcs_m_vals :: "fc_m_vals list"
-
-definition config_m_vals_agree :: "config_m_vals \<Rightarrow> config \<Rightarrow> bool" where
- "config_m_vals_agree v cfg = (case cfg of Config d s fc fcs \<Rightarrow> 
-    s_m_vals_agree (s_m_vals v) s 
-  \<and> fc_m_vals_agree (fc_m_vals v) fc 
-  \<and> list_all2 fc_m_vals_agree (fcs_m_vals v) fcs 
-)"
-
-definition config_m_assn :: "config_m_vals \<Rightarrow> config_m \<Rightarrow> assn" where 
- "config_m_assn v cfg_m = (case cfg_m of Config_m d s_m fc_m fcs_m \<Rightarrow> 
-    s_m_assn (s_m_vals v) s_m 
-  * fc_m_assn (fc_m_vals v) fc_m 
-  * list_assn fc_m_assn (fcs_m_vals v) fcs_m
-)" 
-
-definition vals_of_config_m :: "heap \<Rightarrow> config_m \<Rightarrow> (config_m_vals \<times> addr set) option" where 
- "vals_of_config_m h cfg_m = (case cfg_m of Config_m d s_m fc_m fcs_m \<Rightarrow>
-  vals_of_s_m h s_m \<bind> 
-  (\<lambda> (s_m_vals, s_addrs). vals_of_fc_m h fc_m \<bind> 
-  (\<lambda> (fc_m_vals, fc_addrs). those (map (vals_of_fc_m h) fcs_m) \<bind> 
-  (\<lambda> fcs_v_a.  
-  let fcs_m_vals = map fst fcs_v_a in 
-  let fcs_addrs = map snd fcs_v_a in 
-  Union_of_disjoint (s_addrs#fc_addrs#fcs_addrs) \<bind> 
-  (\<lambda> addrs. 
-   Some (\<lparr>s_m_vals = s_m_vals, fc_m_vals = fc_m_vals, fcs_m_vals = fcs_m_vals\<rparr>, addrs) 
-  )))))"
-
-lemma config_m_vals_sound_assn: 
-  assumes "Some (v, as) = vals_of_config_m h cfg_m" 
-  shows "(h, as) \<Turnstile> config_m_assn v cfg_m" 
-  using assms s_m_vals_sound_assn fc_m_vals_sound_assn 
-  unfolding config_m_assn_def vals_of_config_m_def 
-  apply(simp split:config_m.splits prod.splits) sorry
-
-lemma config_m_vals_sound_agree: 
-  assumes "Some (v, as) = vals_of_config_m h cfg_m" 
-  shows "config_m_vals_agree v (config_m_to_config h cfg_m)"
-  using assms s_m_vals_sound_agree 
-  unfolding vals_of_config_m_def config_m_vals_agree_def config_m_to_config_def
-  apply(simp split: config_m.splits prod.splits config.splits) sorry
-
-lemma config_m_preservation:
-  assumes "config_m_vals_agree v cfg" "(h, as) \<Turnstile> config_m_assn v cfg_m " 
-  shows "cfg = config_m_to_config h cfg_m" 
-  sorry
-
-lemma config_m_vals_update_step_m:
-  assumes "cfg_m' = (Config_m d s (update_fc_step_m fc v_s' es_cont) fcs)"
-  shows "vals_of_config_m h cfg_m'
-    = vals_of_config_m h (Config_m d s fc fcs)"
-  using assms fc_m_vals_update_step_m unfolding vals_of_config_m_def  
-  by(simp split: config_m.splits)
-
-lemma insert_pure: 
-  assumes "<P> f <\<lambda>r. \<up>(Q r) * true>" "<P> f <\<lambda>r. R r>"
-  shows "<P> f <\<lambda>r.  \<up>(Q r) * R r>"
-  using assms
-  by (smt (verit, ccfv_threshold) hoare_triple_def lambda_one pure_false pure_true star_false_left) 
-
 lemmas splits = 
   frame_context_m.splits frame_context.splits config_m.splits redex.splits prod.splits
 
@@ -396,22 +201,25 @@ lemmas defs =
   Heap_Monad.return_def Heap_Monad.heap_def 
   config_m_to_config_def frame_context_m_to_frame_context_def
 
+definition cfg_m_assn :: "config \<Rightarrow> config_m \<Rightarrow> assn" where
+  "cfg_m_assn cfg cfg_m = false"
 
-lemma nth_emp:"<emp> Array.nth a i <\<lambda>r. emp>" 
-  unfolding hoare_triple_def
-  using in_range.simps relH_def run_nth by fastforce
+abbreviation cfg_m_pair_assn where 
+  "cfg_m_pair_assn p p_m \<equiv> 
+  let (cfg, res) = p in 
+  let (cfg_m, res_m) = p_m in 
+  cfg_m_assn cfg cfg_m * \<up>(res = res_m)"
 
-lemma len_emp:"<emp> Array.len a <\<lambda>r. emp>" 
-  unfolding hoare_triple_def
-  using in_range.simps relH_def run_length by fastforce
+lemma run_step_b_e_m_triple:
+    "<cfg_m_assn cfg cfg_m> run_step_b_e_m b_e cfg_m 
+    <\<lambda>r. cfg_m_pair_assn (run_step_b_e b_e cfg) r>"
+  sorry
 
 lemma run_step_b_e_m_run_step_b_e:
   assumes 
-    "vals_of_config_m h cfg_m \<noteq> None"
     "execute (run_step_b_e_m b_e cfg_m) h = Some ((cfg_m', res), h')"
   shows 
-    "run_step_b_e b_e (config_m_to_config h cfg_m) = ((config_m_to_config h' cfg_m'), res)
-    \<and> vals_of_config_m h' cfg_m' \<noteq> None"
+    "run_step_b_e b_e (config_m_to_config h cfg_m) = ((config_m_to_config h' cfg_m'), res)"
   using assms
 proof - 
   define cfg where "cfg = config_m_to_config h cfg_m"
@@ -450,69 +258,27 @@ proof -
       using assms unfolding Current_memory 1 execute_bind_case 
       by(simp add:execute_simps split: option.splits prod.splits)
 
-    obtain v as where v_def:"Some (v, as) = vals_of_config_m h cfg_m" using assms(1)
-      by force
-       
-    have pre1:"(h, as) \<Turnstile> config_m_assn v cfg_m" using config_m_vals_sound_assn[OF v_def] by -
-
-    have pre2:"config_m_vals_agree v cfg" using config_m_vals_sound_agree[OF v_def] cfg_def by auto
-
-    have mem_size_triple1:"<config_m_assn v cfg_m * \<up>(config_m_vals_agree v cfg)> 
-          app_s_f_v_s_mem_size_m (s_m.mems s_m) f_inst2 v_s 
-          <\<lambda>r. \<up>(r = app_s_f_v_s_mem_size (s.mems s) f v_s) * true>"
-      apply(rule hoare_triple_preI) 
-      sorry
-
-    have mem_size_triple15:"<emp> app_s_f_v_s_mem_size_m (s_m.mems s_m) f_inst2 v_s <\<lambda>r. emp>"
-    proof - 
-      show ?thesis
-        unfolding app_s_f_v_s_mem_size_m_def
-        apply(rule bind_rule[OF nth_emp])
-        apply(rule bind_rule[OF nth_emp])
-        apply(rule bind_rule[OF len_emp])
-        by(rule Hoare_Triple.return_wp_rule)
-    qed
-
-    have mem_size_triple2:"<config_m_assn v cfg_m * \<up>(config_m_vals_agree v cfg)> 
-          app_s_f_v_s_mem_size_m (s_m.mems s_m) f_inst2 v_s 
-          <\<lambda>r. config_m_assn v cfg_m * \<up>(config_m_vals_agree v cfg)>"
-      using frame_rule[OF mem_size_triple15] by auto
-
-    have "(h', new_addrs h as h') \<Turnstile> \<up>((v_s'_m, res) = app_s_f_v_s_mem_size (s.mems s) f v_s) * true"
-      using hoare_triple_effect[OF mem_size_triple1] pre1 pre2 mem_size_m 
-      unfolding success_def effect_def
-      by force
-
-    then have "(v_s'_m, res) = app_s_f_v_s_mem_size (s.mems s) f v_s" by auto 
+    have "h' = h" using mem_size_m 
+      sorry 
+      
+    then have "(v_s'_m, res) = app_s_f_v_s_mem_size (s.mems s) f v_s" sorry 
     then have 2:"v_s' = v_s'_m \<and> res = res'" using mem_size prod.inject by metis
-
-    have "(h', new_addrs h as h') \<Turnstile> config_m_assn v cfg_m * \<up>(config_m_vals_agree v cfg)"
-      using hoare_triple_effect[OF mem_size_triple2] pre1 pre2 mem_size_m 
-      unfolding success_def effect_def
-      by force
-
-    then have 3:"cfg = config_m_to_config h' cfg_m" using config_m_preservation by auto
-
-    have 4:"fc = frame_context_m_to_frame_context h' fc_m" 
-      using 3 config config_m unfolding cfg_def config_m_to_config_def 
-      by (simp split: config_m.splits)
 
     have "Config d s (update_fc_step fc v_s' []) fcs = config_m_to_config h' cfg_m'"
     proof -
-      have "s = s_m_to_s h' s_m" using 3 config config_m unfolding cfg_def config_m_to_config_def 
+      have "fc = frame_context_m_to_frame_context h' fc_m" 
+        using \<open>h' = h\<close> config config_m unfolding cfg_def config_m_to_config_def 
         by (simp split: config_m.splits)
-      moreover have "update_fc_step fc v_s' [] 
-        = frame_context_m_to_frame_context h' (update_fc_step_m fc_m v_s'_m [])" 
-        using 4 2 unfolding frame_context_m_to_frame_context_def 
+      then have 
+        "update_fc_step fc v_s' [] = frame_context_m_to_frame_context h' (update_fc_step_m fc_m v_s'_m [])" 
+        using 2 unfolding frame_context_m_to_frame_context_def 
         by(simp split: frame_context.splits frame_context_m.splits)
-      moreover have "fcs = map (frame_context_m_to_frame_context h') fcs_m" 
-        using 3 config config_m unfolding cfg_def config_m_to_config_def 
-        by (simp split: config_m.splits, auto)
-      ultimately show ?thesis unfolding config_m_to_config_def cfg_m'
-        by(simp split: config_m.splits)
+      then show ?thesis using config unfolding \<open>h' = h\<close> config_m_to_config_def cfg_m'
+        by(simp add:config_m split: config_m.splits)
     qed
-    moreover have "res' = res" using 2 by auto
-    ultimately show ?thesis using step_b_e Current_memory sorry
+    then show ?thesis using 2 step_b_e Current_memory assms(1) 
+      unfolding \<open>h' = h\<close> config_m
+      sorry
   next
     case (Call k)
     show ?thesis using assms unfolding Call 
@@ -543,87 +309,13 @@ proof -
     case Grow_memory
     then show ?thesis sorry
   next
-    case Unreachable show ?thesis using assms by (auto simp add: defs Unreachable split: splits)
-  next
-    case Nop show ?thesis using assms by (auto simp add: defs Nop split: splits)
-  next
-    case Drop
-    obtain v_s' where 1:"cfg_m' = Config_m d s_m (update_fc_step_m fc_m v_s' []) fcs_m"
-      using assms by (auto simp add: defs Drop config_m split: splits) 
-    show ?thesis using assms config_m_vals_update_step_m[OF 1] config_m
-      by (auto simp add: defs Drop split: splits)
-  next
-    case Select 
-    obtain v_s' where 1:"cfg_m' = Config_m d s_m (update_fc_step_m fc_m v_s' []) fcs_m"
-      using assms by (auto simp add: defs Select config_m split: splits) 
-    show ?thesis using assms config_m_vals_update_step_m[OF 1] config_m
-      by (auto simp add: defs Select split: splits)
-  next
     case (Block tf b_ebs)
     show ?thesis using assms unfolding Block 
-      sorry
-      (*apply (auto simp add: defs Let_def split: splits tf.split)*)
+      by (auto simp add: defs Let_def split: splits tf.split)
   next
     case (Loop tf b_els)
     show ?thesis using assms unfolding Loop 
-      sorry
-      (*apply (auto simp add: defs Let_def split: splits tf.split)*)
-  next
-    case (If tf es1 es2) 
-    obtain v_s' es_cont where 1:"cfg_m' = Config_m d s_m (update_fc_step_m fc_m v_s' es_cont) fcs_m"
-      using assms by (auto simp add: defs If config_m split: splits) 
-    show ?thesis using assms config_m_vals_update_step_m[OF 1] config_m
-      by (auto simp add: defs If split: splits)
-  next
-    case (Br_if k)
-    obtain v_s' es_cont where 1:"cfg_m' = Config_m d s_m (update_fc_step_m fc_m v_s' es_cont) fcs_m"
-      using assms by (auto simp add: defs Br_if config_m split: splits) 
-    show ?thesis using assms config_m_vals_update_step_m[OF 1] config_m
-      by (auto simp add: defs Br_if split: splits)
-  next
-    case (Br_table ks k) 
-    obtain v_s' es_cont where 1:"cfg_m' = Config_m d s_m (update_fc_step_m fc_m v_s' es_cont) fcs_m"
-      using assms by (auto simp add: defs Br_table config_m split: splits) 
-    show ?thesis using assms config_m_vals_update_step_m[OF 1] config_m
-      by (auto simp add: defs Br_table split: splits)
-  next
-    case (Tee_local k) 
-    obtain v_s' es_cont where 1:"cfg_m' = Config_m d s_m (update_fc_step_m fc_m v_s' es_cont) fcs_m"
-      using assms by (auto simp add: defs Tee_local config_m split: splits) 
-    show ?thesis using assms config_m_vals_update_step_m[OF 1] config_m
-      by (auto simp add: defs Tee_local split: splits)
-  next
-    case (EConst k) show ?thesis using assms by (auto simp add: defs EConst split: splits)
-  next
-    case (Unop t op) 
-    obtain v_s' where 1:"cfg_m' = Config_m d s_m (update_fc_step_m fc_m v_s' []) fcs_m"
-      using assms by (auto simp add: defs Unop config_m split: splits) 
-    show ?thesis using assms config_m_vals_update_step_m[OF 1] config_m
-      by (auto simp add: defs Unop split: splits)
-  next
-    case (Binop t op) 
-    obtain v_s' where 1:"cfg_m' = Config_m d s_m (update_fc_step_m fc_m v_s' []) fcs_m"
-      using assms by (auto simp add: defs Binop config_m split: splits) 
-    show ?thesis using assms config_m_vals_update_step_m[OF 1] config_m
-      by (auto simp add: defs Binop split: splits)  
-  next
-    case (Testop t op) 
-    obtain v_s' where 1:"cfg_m' = Config_m d s_m (update_fc_step_m fc_m v_s' []) fcs_m"
-      using assms by (auto simp add: defs Testop config_m split: splits) 
-    show ?thesis using assms config_m_vals_update_step_m[OF 1] config_m
-      by (auto simp add: defs Testop split: splits)
-  next
-    case (Relop t op)     
-    obtain v_s' where 1:"cfg_m' = Config_m d s_m (update_fc_step_m fc_m v_s' []) fcs_m"
-      using assms by (auto simp add: defs Relop config_m split: splits) 
-    show ?thesis using assms config_m_vals_update_step_m[OF 1] config_m
-      by (auto simp add: defs Relop split: splits)
-  next
-    case (Cvtop t2 op t1 sx) 
-    obtain v_s' where 1:"cfg_m' = Config_m d s_m (update_fc_step_m fc_m v_s' []) fcs_m"
-      using assms by (auto simp add: defs Cvtop config_m split: splits) 
-    show ?thesis using assms config_m_vals_update_step_m[OF 1] config_m
-      by (auto simp add: defs Cvtop split: splits)
+      by (auto simp add: defs Let_def split: splits tf.split)
   next
     case Return
     (* why are those defined twice? *)
@@ -632,29 +324,54 @@ proof -
       by (metis Wasm_Interpreter.update_redex_return.elims 
           Wasm_Interpreter_Monad.update_redex_return.simps)
     show ?thesis using assms unfolding Return 
-      sorry
-      (*by (auto simp add: defs 1 split: splits frame_context_m.split list.split)*)
+      by (auto simp add: defs 1 split: splits frame_context_m.split list.split)
   next
     case (Br k)
     show ?thesis using assms unfolding Br
-      sorry
-      (*by (auto simp add: defs Let_def split: splits label_context.splits if_splits)*)
-  qed
+      by (auto simp add: defs Let_def split: splits label_context.splits if_splits)
+  next
+    case Unreachable show ?thesis using assms by (auto simp add: defs Unreachable split: splits)
+  next
+    case Nop show ?thesis using assms by (auto simp add: defs Nop split: splits)
+  next
+    case Drop show ?thesis using assms by (auto simp add: defs Drop split: splits)
+  next
+    case Select show ?thesis using assms by (auto simp add: defs Select split: splits)
+  next
+    case (If tf es1 es2) show ?thesis using assms by (auto simp add: defs If split: splits)
+  next
+    case (Br_if k) show ?thesis using assms  by (auto simp add: defs Br_if split: splits)
+  next
+    case (Br_table ks k) show ?thesis using assms by (auto simp add: defs Br_table split: splits)
+  next
+    case (Tee_local k) show ?thesis using assms by (auto simp add: defs Tee_local split: splits)
+  next
+    case (EConst k) show ?thesis using assms by (auto simp add: defs EConst split: splits)
+  next
+    case (Unop t op) show ?thesis using assms by (auto simp add: defs Unop split: splits)
+  next
+    case (Binop t op) show ?thesis using assms by (auto simp add: defs Binop split: splits)  
+  next
+    case (Testop t op) show ?thesis using assms by (auto simp add: defs Testop split: splits)
+  next
+    case (Relop t op) show ?thesis using assms by (auto simp add: defs Relop split: splits)
+  next
+    case (Cvtop t2 op t1 sx) show ?thesis using assms by (auto simp add: defs Cvtop split: splits)
+  qed 
 qed 
+
 lemma run_step_e_m_run_step_e:
   assumes 
-    "vals_of_config_m h cfg_m \<noteq> None"
     "execute (run_step_e_m e cfg_m) h = Some ((cfg_m', res), h')"
   shows 
-    "run_step_e e (config_m_to_config h cfg_m) = ((config_m_to_config h' cfg_m'), res) 
-  \<and> vals_of_config_m h' cfg_m' \<noteq> None"
+    "run_step_e e (config_m_to_config h cfg_m) = ((config_m_to_config h' cfg_m'), res)"
 proof(cases e)
   case (Basic b_e)
   have 1:"run_step_e_m e cfg_m = run_step_b_e_m b_e cfg_m" unfolding Basic
     by(rule config_m.induct, auto simp add: defs split: splits)
   have "run_step_e e (config_m_to_config h cfg_m) = run_step_b_e b_e (config_m_to_config h cfg_m)"
     unfolding Basic by(rule config.induct, auto simp add: defs split: splits) 
-  also have "... = ((config_m_to_config h' cfg_m'), res) \<and> vals_of_config_m h' cfg_m' \<noteq> None" 
+  also have "... = ((config_m_to_config h' cfg_m'), res)" 
     using assms run_step_b_e_m_run_step_b_e unfolding 1 by simp
   finally show ?thesis by -
 next
